example.v
@@ -1,0 +1,161 @@
+From SMTCoq Require Import SMTCoq.
+From SMTCoq Require Import PArray Int63.
+Require Import GCHQ.
+Import Datatypes.
+
+Notation "'X'"  := (id true).
+
+Notation "'O'"  := (id false).
+
+Definition sol_pb1 := 
+(
+ (O :: O :: O :: O :: O :: O :: O :: X :: O :: O :: O :: X :: X :: X :: O :: X :: O :: X :: O :: O :: O :: O :: O :: O :: O :: nil) ::
+ (O :: X :: X :: X :: X :: X :: O :: X :: O :: O :: X :: O :: O :: X :: X :: X :: X :: X :: O :: X :: X :: X :: X :: X :: O :: nil) ::
+ (O :: X :: O :: O :: O :: X :: O :: X :: X :: X :: X :: X :: O :: O :: O :: X :: O :: X :: O :: X :: O :: O :: O :: X :: O :: nil) ::
+ (O :: X :: O :: O :: O :: X :: O :: X :: O :: X :: X :: O :: O :: O :: O :: O :: O :: X :: O :: X :: O :: O :: O :: X :: O :: nil) ::
+ (O :: X :: O :: O :: O :: X :: O :: X :: X :: O :: O :: O :: O :: O :: X :: O :: O :: X :: O :: X :: O :: O :: O :: X :: O :: nil) ::
+ (O :: X :: X :: X :: X :: X :: O :: X :: X :: O :: O :: X :: X :: X :: X :: X :: X :: X :: O :: X :: X :: X :: X :: X :: O :: nil) ::
+ (O :: O :: O :: O :: O :: O :: O :: X :: O :: X :: O :: X :: O :: X :: O :: X :: O :: X :: O :: O :: O :: O :: O :: O :: O :: nil) ::
+ (X :: X :: X :: X :: X :: X :: X :: X :: O :: O :: O :: X :: X :: X :: O :: O :: O :: X :: X :: X :: X :: X :: X :: X :: X :: nil) ::
+ (O :: X :: O :: O :: X :: O :: O :: O :: X :: X :: O :: X :: O :: X :: O :: O :: O :: X :: O :: X :: X :: O :: X :: O :: O :: nil) ::
+ (O :: X :: O :: X :: X :: X :: X :: X :: X :: O :: O :: O :: X :: O :: O :: X :: X :: X :: X :: O :: X :: X :: X :: O :: X :: nil) ::
+ (X :: O :: O :: O :: O :: X :: O :: X :: O :: O :: O :: O :: X :: O :: O :: X :: O :: X :: X :: X :: X :: O :: O :: X :: X :: nil) ::
+ (X :: O :: X :: O :: X :: X :: X :: O :: X :: X :: X :: O :: X :: O :: X :: O :: O :: O :: O :: X :: O :: X :: O :: O :: O :: nil) ::
+ (X :: X :: O :: O :: X :: X :: O :: X :: O :: X :: O :: X :: X :: X :: X :: X :: X :: O :: O :: X :: O :: O :: O :: O :: O :: nil) ::
+ (X :: X :: X :: O :: O :: O :: X :: O :: O :: X :: O :: O :: X :: O :: O :: O :: O :: O :: O :: X :: O :: O :: O :: X :: O :: nil) ::
+ (O :: X :: O :: O :: O :: O :: O :: O :: O :: O :: O :: X :: O :: X :: O :: X :: X :: O :: O :: X :: X :: X :: X :: O :: X :: nil) ::
+ (X :: O :: O :: X :: O :: X :: X :: O :: O :: X :: X :: X :: O :: O :: X :: O :: O :: O :: X :: X :: X :: X :: X :: O :: X :: nil) ::
+ (O :: O :: O :: X :: O :: X :: O :: X :: O :: X :: X :: O :: X :: X :: X :: X :: O :: O :: O :: O :: O :: X :: O :: X :: X :: nil) ::
+ (X :: X :: X :: X :: X :: X :: X :: X :: O :: X :: X :: X :: O :: O :: X :: O :: O :: X :: X :: X :: O :: O :: O :: O :: O :: nil) ::
+ (O :: O :: O :: O :: O :: O :: O :: X :: O :: X :: X :: O :: O :: X :: X :: X :: O :: X :: O :: X :: O :: X :: O :: O :: O :: nil) ::
+ (O :: X :: X :: X :: X :: X :: O :: X :: O :: O :: X :: X :: O :: X :: X :: O :: O :: X :: X :: X :: O :: O :: X :: O :: X :: nil) ::
+ (O :: X :: O :: O :: O :: X :: O :: X :: X :: X :: O :: O :: O :: O :: X :: X :: O :: O :: O :: O :: O :: X :: X :: O :: X :: nil) ::
+ (O :: X :: O :: O :: O :: X :: O :: X :: O :: O :: O :: X :: O :: O :: O :: O :: O :: O :: O :: O :: O :: O :: X :: O :: O :: nil) ::
+ (O :: X :: O :: O :: O :: X :: O :: X :: O :: X :: X :: O :: O :: O :: O :: O :: O :: X :: O :: O :: O :: O :: O :: O :: X :: nil) ::
+ (O :: X :: X :: X :: X :: X :: O :: X :: X :: O :: O :: X :: X :: X :: X :: X :: X :: O :: X :: O :: X :: O :: O :: X :: X :: nil) ::
+ (O :: O :: O :: O :: O :: O :: O :: X :: O :: O :: X :: X :: X :: O :: X :: O :: O :: X :: X :: X :: O :: O :: O :: O :: O :: nil) :: nil
+).
+
+Lemma verify_sol_pb1 : verify_sol pb1 sol_pb1.
+Proof. by compute. Qed.
+
+Lemma interp_free f u : 
+  interp f u =
+   let ff f := finterp u (fun x => f (to_Z x))
+   in ff (fun x => f (Int63Op.of_Z x))
+   true false 
+  Bool.eqb mk_andb mk_implb mk_orb Datatypes.negb.
+Proof.
+simpl.
+apply interp_ext; intro x.
+by rewrite Int63Axioms.of_to_Z.
+Qed.
+
+
+Lemma sol_pb1_ok s : verify_sol pb1 s -> sol_pb1 = s.
+Proof.
+intro H.
+apply (test_eq_correct pb1).
+- by compute.
+- by compute.
+- by compute.
+- by apply verify_sol_pb1.
+- by exact H.
+rewrite interp_free.
+set (u := fun _ =>  _).
+vm_compute in u.
+set (ff := (fun _ => _)).
+unfold u.
+   lazy delta[is_true mk_andb mk_orb mk_implb 
+     seq.head seq.foldl seq.foldr seq.behead] iota beta.
+unfold is_true.
+verit.
+Qed.
+
+
+(*
+Definition pb := pb2.
+Definition es : sol := nil.
+Definition tr (z : Z) := true.
+
+
+Time Definition tt1 f :=
+   Eval vm_compute in  finterp (gen_all pb) (fun x => f (to_Z x)).
+
+
+Time Definition tt2 :=
+  Eval lazy delta[tt1 mk_andb mk_orb 
+     seq.head seq.foldl seq.behead] iota beta in 
+  tt1 tr true false 
+  Bool.eqb mk_andb mk_implb mk_orb Datatypes.negb.
+
+Ltac end_tac v :=
+  let w := eval compute in v in
+idtac w;
+(timeout 40 (
+    try (
+     assert (Datatypes.implb tt2 ((tr w))); [
+                          unfold tt2; verit | idtac]; 
+                                  idtac "ho"; fail 1);
+      idtac "false"; exact false)) ||
+idtac "true"; exact true.
+
+Ltac col i j n :=
+  let u := constr:(Zeq_bool j n) in 
+  let v := eval compute in u in
+     match v with true => exact nil
+                 |false => apply cons; 
+                           [end_tac (i * n + j)%Z|
+                            col i (j + 1)%Z n]
+     end.
+
+Ltac row i n :=
+  let u := constr:(Zeq_bool i n) in 
+  let v := eval compute in u in
+     match v with true => exact nil
+                 |false => apply cons; 
+                           [col i 0%Z n|
+                            row (i + 1)%Z n]
+     end.
+
+Definition s : sol.
+row 0 (Z.of_nat (p_size pb)).
+Defined.
+
+Lemma verify_sol_s : verify_sol pb s.
+Proof. by compute. Qed.
+
+Lemma interp_free f u : 
+  interp f u =
+   let ff f := finterp u (fun x => f (to_Z x))
+   in ff (fun x => f (Int63Op.of_Z x))
+   true false 
+  Bool.eqb mk_andb mk_implb mk_orb Datatypes.negb.
+Proof.
+simpl.
+apply interp_ext; intro x.
+by rewrite Int63Axioms.of_to_Z.
+Qed.
+
+
+Lemma s_ok s1 : verify_sol pb s1 -> s = s1.
+
+Proof.
+intro H.
+apply (test_eq_correct pb).
+- by compute.
+- by compute.
+- by compute.
+- by apply verify_sol_s.
+- by exact H.
+rewrite interp_free.
+set (u := fun _ =>  _).
+compute in u.
+set (ff := (fun _ => _)).
+unfold u.
+   lazy delta[is_true mk_andb mk_orb mk_implb 
+     seq.head seq.foldl seq.foldr seq.behead] iota beta.
+verit.
+Qed.
+
+*)
